theories/Dot/examples/typingExInfra.v
@@ -23,8 +23,8 @@ Notation s2 := (2 %positive).
 Notation "'type' l = ( σ ; s )" := (l, dtysem σ s) (at level 60, l at level 50).
 
 Check ν {@ type "A" = (σ1 ; s1) }.
-Check ν {@ val "a" = vnat 0; type "A" = (σ1 ; s1) }.
-Check ν {@ val "a" = vnat 0 ; type "A" = (σ1 ; s1) }.
+Check ν {@ val "a" = pv (vnat 0); type "A" = (σ1 ; s1) }.
+Check ν {@ val "a" = pv (vnat 0) ; type "A" = (σ1 ; s1) }.
 
 (***************)
 (** WEAKENING **)
